Denote function for Choice

src/Choice.v
@@ -31,17 +31,26 @@ Class Computes (s : Type) (eff : Type -> Type) := {
 
 Arguments computes {s eff _ a} _ _ _ _.
 
-
 Require Import Eff.
 
 Class Denotes (v : Type) (effs : list (Type -> Type)) := {
-  denotes : forall a, Eff effs a -> v -> Prop
+  denotes : Eff effs v -> v -> Prop
 }.
 
-Arguments denotes {v effs _ _} _ _.
+Arguments denotes {v effs _} _ _.
 
-Definition denotes' v a : Eff [Comp] a -> v -> Prop :=
-  fun st _ => False.
+
+Program Instance Comp_Denotes {s}: Denotes s [Comp] :=
+  {
+    denotes := fun (st: Eff [Comp] s) v =>
+                 match st with
+                 | Pure x => x = v
+                 | @Impure _ _ x fx c => _
+                 end
+  }.
+Next Obligation.
+Admitted.
+
 
 (* Given an interpreter that can run any effect down to its denotation in
    Gallina, we can interpret any action. *)
