src/Refine2.v
@@ -1,0 +1,137 @@
+Require Export Imp.
+Require Import
+  Coq.Program.Program
+  Coq.Program.Tactics
+  Coq.omega.Omega
+  Coq.Lists.List.
+
+Require Export
+  Eff
+  Comp
+  Choice.
+
+Import ListNotations.
+
+Generalizable All Variables.
+
+Require Import
+  Hask.Control.Monad
+  RWS.
+
+Definition nonDet_list : Eff [Choice] (list nat) :=
+  (l <- send (Pick (fun (l: list nat) => (length l) >= 10));
+     pure l).
+
+Definition det_list: Eff [Choice] _ :=
+     (pure (repeat 10 11)).
+
+Program Fixpoint denotes_choice {v} (s1: Eff [Choice] v) (s2: Eff [] v): Prop :=
+  match s2 with
+  | Impure u _ => False_rect _ (Union_empty _ u)
+  | Pure a2 =>
+    match s1 with
+    | Pure a1 => a1 = a2
+    | Impure u1 k =>
+      match extract u1 with
+      | Pick p => exists a, denotes_choice (k a) s2 /\ p a
+      end
+    end
+  end.
+
+
+Program Fixpoint denotes {v} (s1: Eff [Comp] v): Eff [] v -> Prop :=
+  fun s2 => match s2 with
+  | Impure u _ => False_rect _ (Union_empty _ u)
+  | Pure a2 =>
+    match s1 with
+    | Pure a1 => a1 = a2
+    | Impure u1 k =>
+      match extract u1 with
+      | p => exists a, denotes (k a) s2 /\ p a
+      end
+    end
+  end.
+
+Lemma reduce_nonDet: 
+  denotes_choice nonDet_list (pure (repeat 10 11)).
+Proof.
+  intros.
+  remember (repeat 10 11) as l.
+  simpl.
+  exists l.
+  subst; split; simpl; auto.
+Qed.
+
+Lemma nonEffect_Denotes: forall v (l: v),
+    denotes_choice (pure l) (pure l).
+Proof.
+  reflexivity.
+Qed.
+
+Lemma nonEffect_pure: forall v (l: v) x,
+    denotes_choice (pure l) x -> x = (pure l).
+Proof.
+  intros.
+  simpl in *.
+  destruct x eqn:Heq in *; subst; auto.
+  inversion u.
+Qed.
+
+Lemma pure_nonEffect: forall v (l: v) x,
+    x = (pure l) -> denotes_choice (pure l) x.
+Proof.
+  intros.
+  simpl in *.
+  destruct x eqn:Heq in *; subst; auto.
+  inversion H; auto.
+  inversion u.
+Qed.
+
+(* e1 refines e2 if forall t \in [| e2 |] -> t \in [| e1 |] *)
+Definition refines {v} e1 e2 := forall t, @denotes_choice v e2 t -> @denotes_choice v e1 t.
+
+Lemma refines_detList_nonDetList:
+    refines nonDet_list det_list.
+Proof.
+  intros t H.
+  apply nonEffect_pure in H.
+  subst.
+  apply reduce_nonDet.
+Qed.
+
+Fixpoint pack_aexp (st: state) (a:aexp): Eff [Comp] nat :=
+  match a with
+  | ANum n => pure n
+  | AId x => Impure (@UThis _ Comp _ (fun n => st x = n))
+                   (fun n => pure n)
+  | APlus a1 a2 | AMinus a1 a2 | AMult a1 a2
+                                 => pack_aexp st a1 ;; pack_aexp st a2
+  end.
+
+Fixpoint pack_bexp (st: state) (b:bexp): Eff [Comp] bool :=
+  match b with
+  | BTrue => pure true
+  | BFalse => pure false
+  | BEq a1 a2 | BLe a1 a2 => (x1 <- (pack_aexp st a1) ;
+                               x2 <- (pack_aexp st a2) ;
+                               pure (beq_nat x1 x2))
+  | BAnd b1 b2 => (x1 <- pack_bexp st b1;
+                    x2 <- pack_bexp st b2;
+                    pure (andb x1 x2))
+  | BNot b' => (b'' <- pack_bexp st b';
+                 pure (negb b''))
+  end.
+
+Fixpoint pack_imp (st: state) (c: com): Eff [Comp] state :=
+  match c with
+  | SKIP => pure st
+  | CAss x ax => (a <- pack_aexp st ax;
+                   pure (t_update st x a))
+  | IFB b THEN c1 ELSE c2 FI => (b' <- pack_bexp st b;
+                                  c1' <- pack_imp st c1;
+                                  c2' <- pack_imp st c2;
+                                  pure (if b' then c1' else c2'))
+  | c1 ;;; c2 => pack_imp st c1 ;; pack_imp st c2
+  | WHILE b DO c' END => pure st
+  end.
+
