src/Union.v
@@ -9,7 +9,6 @@ Import ListNotations.
 Generalizable All Variables.
 Set Primitive Projections.
 Set Universe Polymorphism.
-Unset Transparent Obligations.
 
 Inductive UnionF (a : Type) : list (Type -> Type) -> Type :=
   | UThis : forall t r, t a -> UnionF a (t :: r)
@@ -34,6 +33,8 @@ Program Definition decomp `(u : Union (t :: r) v) : t v + Union r v :=
   | UThis x => fun _ => inl (_ x)
   | UThat x => fun _ => inr x
   end eq_refl.
+Unset Transparent Obligations.
+
 
 Definition decomp_rev `(u : Union (r ++ [t]) v) : Union r v + t v.
 Proof.
@@ -50,7 +51,7 @@ Defined.
 
 Program Definition extract `(u : Union [t] v) : t v :=
   match decomp u with | inl x => x | inr x => ! end.
-Next Obligation. inversion x. Qed.
+Next Obligation. inversion x. Defined.
 
 Definition weaken {t} `(u : Union r v) : Union (t :: r) v := UThat u.
 
